pcuic/theories/PCUICInductiveInversion.v
@@ -2355,28 +2355,6 @@ Proof.
   rewrite !subst_closedn //.
 Qed.
 
-Lemma subst_instance_expand_lets u Γ t :
-  subst_instance u (expand_lets Γ t) = 
-  expand_lets (subst_instance u Γ) (subst_instance u t).
-Proof.
-  rewrite /expand_lets /expand_lets_k.
-  rewrite subst_instance_subst.
-  rewrite subst_instance_extended_subst.
-  f_equal.
-  rewrite subst_instance_lift. len; f_equal.
-Qed.
-
-Hint Rewrite subst_instance_expand_lets closedn_subst_instance : substu.
-
-Lemma subst_instance_expand_lets_ctx u Γ Δ :
-  subst_instance u (expand_lets_ctx Γ Δ) =
-  expand_lets_ctx (subst_instance u Γ) (subst_instance u Δ).
-Proof.
-  rewrite /expand_lets_ctx /expand_lets_k_ctx.
-  rewrite !subst_instance_subst_context !subst_instance_lift_context; len.
-  now rewrite -subst_instance_extended_subst.
-Qed.
-
 Lemma into_context_equality_rel {cf} {Σ} {wfΣ : wf Σ} {Γ Δ Δ'}
   (c : cumul_ctx_rel Σ Γ Δ Δ') : 
   is_closed_context (Γ ,,, Δ) ->
